Try to write compilation

io/ModelingLanguage.fst
@@ -9,10 +9,14 @@ open IIO
 noeq type monad = {
   m    : Type u#a -> Type u#(max 1 a);
   ret  : #a:Type -> a -> m a;
-  bind : #a:Type -> #b:Type -> m a -> (a -> m b) -> m b;
 }
 
-let  pi_type = monitorable_prop
+//type mon_bind (mon:monad) = #a:Type u#a -> #b:Type u#b -> mon.m a -> (a -> mon.m b) -> mon.m b
+
+val free : monad
+let free = { m = iio; ret = iio_return; }
+
+let pi_type = monitorable_prop
 
 noeq
 type interface = {
@@ -31,41 +35,58 @@ type acts (mon:monad) = op:io_cmds -> arg:io_sig.args op -> mon.m (io_sig.res op
    I think we need to pass the abstract monad inside is we want to support higher-order types.
    in this case I conflated alpha + beta = ct, and gamma + delta = pt *)
 
-type ct (i:interface) (m:Type->Type) = i.ctx_in -> m i.ctx_out
-type pt (i:interface) (m:Type->Type) = ct i m -> m i.prog_out 
+(** *** Intermediate Lang **)
+type ictx (i:interface) = x:i.ctx_in -> ILang.IIOpi i.ctx_out i.pi
+type iprog (i:interface) = ictx i -> ILang.IIOpi i.prog_out i.pi
+type iwhole (i:interface) = unit -> ILang.IIOpi i.prog_out i.pi
+let ilink (i:interface) (ip:iprog i) (ic:ictx i) : iwhole i = fun () -> ip ic
 
-type ctx (i:interface) = mon:monad -> acts mon -> ct i mon.m
+(** *** Target Lang **)
+type ct (i:interface) (mon:monad) = i.ctx_in -> mon.m i.ctx_out
+type pt (i:interface) (mon:monad) = mon.m i.prog_out 
 
-val free : monad
-let free = {
-  m = iio;
-  ret = iio_return;
-  bind = iio_bind;
-}
+type ctx (i:interface) = mon:monad -> acts mon -> ct i mon
+type prog (i:interface) = ctx i -> pt i free
 
-type prog (i:interface) = ctx i -> pt i free.m
+type whole (i:interface) (mon:monad) = unit -> pt i mon
+let link (i:interface) (p:prog i) (c:ctx i) : whole i free = fun () -> p c
 
-let stuff = string (* TODO: cheating, to be fixed later *)
-assume val check_get_trace : pi_type -> cmd:io_cmds -> io_sig.args cmd -> free.m bool
+(** *** Backtranslate **)
+(* TODO: these will need to be type-classes depending on structure of ct and pt *)
+assume val backtranslate : (#i:interface) -> ct i free -> ictx i
 
-type whole (i:interface) = pt i
+(** *** Compilation **)
+(* TODO: this could be for any mon:monad not for free *)
+val compile_tree : (#a:Type u#c) -> (m:iio a) -> acts free -> iio a
+let rec compile_tree #a m call_cmd =
+  match m with
+  | Return x -> iio_return x
+  | Call GetTrace arg k -> admit ()
+  | Call cmd arg k -> iio_bind #(iio_sig.res cmd arg) #a (call_cmd cmd arg) (fun x -> compile_tree (k x) call_cmd)
+  | Decorated _ _ _ -> admit () 
+  | PartialCall _ _ -> admit ()
 
-val free_acts : acts free
-(** CA: I can not reify here an IO computation because there is no way to prove the pre-condition **)
-let free_acts cmd arg = IO.Sig.Call.iio_call cmd arg
+(* TODO: this needs to be/include IIO pi arrow; which may bring back reification? in compile_whole? on the argument of compile_whole? *)
+let compile (i:interface) (ip:iprog i) (ca:acts free) : prog i = 
+  fun (c:ctx i) -> 
+    let tree : dm_iio i.prog_out (ILang.pi_hist _ i.pi) = 
+      reify (ip (backtranslate (c free ca))) in
+    let tree' : iio i.prog_out = tree in
+    compile_tree #i.prog_out tree' ca 
 
-(** CA: I would like this to be obtained by reifing the compilation of the IO primitives.
-A solution will be to reify IIO.Primitives.dynamic_call.
-Otherwise, we can implement it again here and show equivalence between this 
-implenetation and the compilation **)
-let wrapped_acts (pi:pi_type) : acts free = 
-  fun cmd arg ->
-    free.bind
-      (check_get_trace pi cmd arg)
-      (fun b -> if b then free_acts cmd arg else free.ret #(io_sig.res cmd arg) (Inr Common.Contract_failure))
 
-let link (i:interface) (p:prog i) (c:ctx i) : whole i free.m = p c
+(* now we can better write backtranslate; TODO: but to typecheck it we need parametricity? *)
 
+(** *** soundness *)
+(* forall ip c pi. compile ip `link pi` c ~> t => t \in pi *)
+
+(* Example:
+   ct free.m = alpha -> free.m beta
+   ictx for this = alpha -> IIO beta pi
+*)
+
+
+(** *** Transparency **)
 (* used to state transparency *)
 (* forall p c pi. link_no_check p c ~> t /\ t \in pi => link p c ~> t *)
 (* let link_no_check (p:prog) (c:ctx) : whole = p (c free free_acts) -- TODO: can't write this any more *)
@@ -85,46 +106,6 @@ let link (i:interface) (p:prog i) (c:ctx i) : whole i free.m = p c
 (* new idea, fixed to account for the fact that certain things checked by wrapped_acts are not in pi: *)
 (* forall ip c pi. link (compile ip free_acts) c ~> t /\ t \in pi => link (compile ip (wrapped_acts pi)) c ~> t *)
 
-let ictx (i:interface) = x:i.ctx_in -> ILang.IIOpi i.ctx_out i.pi
-let iwhole (i:interface) = unit -> ILang.IIOpi i.prog_out i.pi
-
-let iprog (i:interface) = ictx i -> iwhole i
-(* TODO: this needs to be/include IIO pi arrow; which may bring back reification? in compile_whole? on the argument of compile_whole? *)
-
-(* TODO: these will need to be type-classes depending on structure of ct and pt *)
-assume val backtranslate : (#i:interface) -> ct i free.m -> ictx i
-
-#set-options "--print_universes"
-
-val compile_tree : (#a:Type u#c) -> (m:iio a) -> (mon:monad) -> acts mon -> mon.m a
-let rec compile_tree #a m mon call_cmd =
-  match m with
-  | Return x -> mon.ret x
-  | Call GetTrace arg k -> admit ()
-  | Call cmd arg k -> mon.bind #(iio_sig.res cmd arg) #a (call_cmd cmd arg) (fun x -> compile_tree (k x) mon call_cmd)
-  | Decorated _ _ _ -> admit () 
-  | PartialCall _ _ -> admit ()
-
-val compile_whole : (#i:interface) -> iwhole i -> pt i free.m
-let compile_whole #i (w:unit -> ILang.IIOpi i.prog_out i.pi) call_cmd : free.m i.prog_out =
-  let tree : dm_iio i.prog_out (ILang.pi_hist _ i.pi) = reify (w ()) in
-  let tree' : iio i.prog_out = tree in
-  compile_tree #i.prog_out tree' free call_cmd
-
-let compile (i:interface) (ip:iprog i) (ca:acts free) : prog i = 
-  fun (c:ctx i) -> compile_whole (ip (backtranslate (c free ca)))
-
-
-(* now we can better write backtranslate; TODO: but to typecheck it we need parametricity? *)
-
-(* soundness *)
-(* forall ip c pi. compile ip `link pi` c ~> t => t \in pi *)
-
-(* Example:
-   ct free.m = alpha -> free.m beta
-   ictx for this = alpha -> IIO beta pi
-*)
-
 assume val alpha : Type0
 assume val beta : Type0
 (* let bt (pi:...) (f : (alpha -> free.m beta)) (a:alpha) : IIO beta pi = *)
@@ -133,3 +114,19 @@ assume val beta : Type0
 (* Possible issue: backtranslation may be difficult if we allow m at arbitrary places,
    while in F* effects are only allowed at the right or arrows;
    make such kleisli arrows the abstraction instead of m? *)
+
+
+val free_acts : acts free
+(** CA: I can not reify here an IO computation because there is no way to prove the pre-condition **)
+let free_acts cmd arg = IO.Sig.Call.iio_call cmd arg
+
+assume val check_get_trace : pi_type -> cmd:io_cmds -> io_sig.args cmd -> free.m bool
+(** CA: I would like this to be obtained by reifing the compilation of the IO primitives.
+A solution will be to reify IIO.Primitives.dynamic_call.
+Otherwise, we can implement it again here and show equivalence between this 
+implenetation and the compilation **)
+let wrapped_acts (pi:pi_type) : acts free = 
+  fun cmd arg ->
+    iio_bind
+      (check_get_trace pi cmd arg)
+      (fun b -> if b then free_acts cmd arg else free.ret #(io_sig.res cmd arg) (Inr Common.Contract_failure))
